theories/Sem/PLogic.v
@@ -1,0 +1,246 @@
+(*
+ * Copyright (C) BedRock Systems Inc. 2019 Gregory Malecha
+ *
+ * SPDX-License-Identifier:AGPL-3.0-or-later
+ *)
+Require Import Coq.Classes.Morphisms.
+Require Import Coq.NArith.BinNat.
+Require Import Coq.ZArith.BinInt.
+Require Import Coq.Strings.String.
+
+From Cpp Require Import Ast.
+
+From Cpp.Sem Require Import Logic Semantics.
+
+(* todo(gmm): these can be moved somewhere more generic *)
+Class Affine (P : mpred) : Prop :=
+{ can_dup : P |-- P ** P }.
+Class Droppable (P : mpred) : Prop :=
+{ can_drop : P |-- empSP }.
+
+
+(* representations are predicates over a location, they should be used to
+ * assert propreties of the heap
+ *)
+Definition Rep : Type := forall addr : val, mpred.
+(* locations are predicates over a location and are used to do address
+ * arithmetic.
+ * - note(gmm): they are always computable from the program except for when
+ *   they use field and the layout of a class is non-standard or when they
+ *   mention local variables.
+ *)
+Record Loc : Type :=
+{ addr_of : forall addr : val, mpred }.
+
+Definition LocEq (l1 l2 : Loc) : Prop :=
+  forall x y, l1.(addr_of) x //\\ l2.(addr_of) y |-- [| x = y |].
+
+Definition _eq (a : val) : Loc :=
+{| addr_of p := [| p = a |] |}.
+Theorem _eq_LocEq : forall a b, LocEq (_eq a) (_eq b) -> a = b.
+Proof. unfold LocEq, _eq. intros.
+       simpl in *.
+       specialize (H a b).
+       admit.
+Admitted.
+
+Definition _local (r : region) (x : ident) : Loc.
+Admitted.
+Axiom _local_det : forall r x, LocEq (_local r x) (_local r x).
+
+Definition _field (f : field) (base : Loc) : Loc.
+Admitted.
+Axiom Proper__field : forall {f}, Proper (LocEq ==> LocEq) (_field f).
+
+Definition _sub (t : type) (i : Z) (base : Loc) : Loc.
+Admitted.
+Axiom Proper__sub : forall t i, Proper (LocEq ==> LocEq) (_sub t i).
+
+(* this represents static_cast *)
+Definition _super (from to : type) (base : Loc) : Loc.
+Admitted.
+Axiom Proper__super : forall from to, Proper (LocEq ==> LocEq) (_super from to).
+
+
+
+
+(*
+(** pointer offsets *)
+Definition field_addr (f : field) (base : val) : Loc := fun ptr =>
+  with_genv (fun g => Exists off : Z,
+      [| offset_of (c:=g) (Tref f.(f_type)) f.(f_name) off |] **
+      [| offset_ptr base off = ptr |]).
+
+(* todo(gmm): i need a way to compute a parent class offset. *)
+Parameter parent_addr : forall (parent derived : globname) (base : val), Loc.
+
+(* address of a local variable *)
+Parameter local_addr : region -> ident -> Loc.
+*)
+
+(* heap points to *)
+(* note(gmm): this needs to support fractional permissions and other features *)
+Parameter ptsto : val -> Rep.
+
+
+
+(* the pointer contains the code *)
+Parameter code_at : Func -> ptr -> mpred.
+(* code_at is freely duplicable *)
+Axiom code_at_dup : forall p f, code_at p f -|- code_at p f ** code_at p f.
+Axiom code_at_drop : forall p f, code_at p f |-- empSP.
+
+Parameter ctor_at : ptr -> Ctor -> mpred.
+Parameter dtor_at : ptr -> Dtor -> mpred.
+
+
+Parameter is_true : val -> bool.
+Axiom is_true_int : forall i,
+    is_true (Vint i) = negb (BinIntDef.Z.eqb i 0).
+
+(* there shouldn't be locals because locals need a spatial ownership (over
+ * the region)
+ * global addresses admit duplication and weakening
+ *)
+Inductive path : Type :=
+| p_done
+| p_dot  (_ : field) (_ : path) (* field offset *)
+| p_cast (from to : type)  (_ : path) (* parent-class offset, i.e. static_cast *)
+| p_sub  (_ : type) (_ : val) (_ : path).
+
+Fixpoint pathD (p : path) (l : Loc) : Loc :=
+  match p with
+  | p_done => l
+  | p_dot f p => pathD p (_field f l)
+  | p_cast from to p => pathD p (_super (drop_qualifiers from) (drop_qualifiers to) l)
+  | p_sub t v p =>
+    {| addr_of a := Exists i : Z,
+         [| Vint i = v |] //\\
+         (pathD p (_sub (drop_qualifiers t) i l)).(addr_of) a |}
+  end.
+
+Require Import Cpp.Auto.Discharge.
+
+Lemma pathD_det : forall p l1 l2,
+    LocEq l1 l2  -> LocEq (pathD p l1) (pathD p l2).
+Proof.
+  induction p; simpl; intros; eauto.
+  { eapply IHp. eapply Proper__field; eauto. }
+  { eapply IHp. eapply Proper__super. eauto. }
+  { red. simpl. intros.
+    rewrite landexistsDL1; eapply lexistsL; intro.
+    rewrite landexistsDL2; eapply lexistsL; intro.
+    unfold only_provable.
+    admit. }
+Admitted.
+
+
+Definition _addr (base : val) (p : path) : Loc :=
+  pathD p (_eq base).
+
+Notation "a @@ b" := (a.(addr_of) b) (at level 30, no associativity).
+
+Theorem _addr_det : forall p b a1 a2,
+    _addr b p @@ a1 ** _addr b p @@ a2 |-- _addr b p @@ a1 ** [| a1 = a2 |].
+Proof. Admitted.
+
+
+(*
+Parameter Affine__addr : forall b p a, Affine (_addr b p a).
+Parameter Droppable__addr : forall b p a, Droppable (_addr b p a).
+*)
+
+Definition _atP (base : val) (p : path) (P : Rep) : mpred :=
+  Exists addr, (_addr base p) @@ addr ** P addr.
+
+
+Definition _at (base : Loc) (P : Rep) : mpred :=
+  Exists addr, base @@ addr ** P addr.
+
+(* this should probably be split up into a bunch of simpler definitions, e.g.
+ * - `tint (size : nat) : N -> Rep`
+ * - `tuint (size : nat) : N -> Rep`
+ * - ...etc...
+ *)
+Definition tprim (ty : type) (v : val) : Rep :=
+  fun addr => ptsto addr v ** [| has_type v (drop_qualifiers ty) |].
+
+Definition uninit (ty : type) : Rep := fun addr =>
+  Exists bits,
+    (* with_genv (fun env => [| size_of env ty size |]) ** *)
+    tprim ty bits addr.
+
+Definition tany (t : type) : Rep := fun addr =>
+  Exists v, [| has_type v t |] ** tprim t v addr.
+
+(* this isn't really necessary, we should simply drop it and write
+ * predicates in this way to start with
+ *)
+Definition tinv {model} (Inv : val -> model -> mpred) (m : model) : Rep :=
+  fun addr => Inv addr m.
+
+Lemma val_uninit : forall t v, tprim t v |-- uninit t.
+Proof. Admitted.
+
+Lemma val_any : forall t v, tprim t v |-- tany t.
+Proof. Admitted.
+
+Definition _at_cancel : forall a (V V' : Rep) P Q,
+    V |-- V' ->
+    P |-- Q ->
+    _at a V ** P |-- _at a V' ** Q.
+Proof. Admitted.
+
+Definition tlocal_at (r : region) (ty : type) (l : ident) (a : val) (v : val) : mpred :=
+  _local r l @@ a **
+  [| has_type a (Tpointer ty) |] **
+  _at (_eq a) (tprim ty v).
+
+Definition tlocal (r : region) (ty : type) (x : ident) (v : val) : mpred :=
+  Exists a, tlocal_at r ty x a v.
+
+Lemma tlocal_at_tlocal : forall r ty x a v F F',
+    F |-- F' ->
+    tlocal_at r ty x a v ** F |-- tlocal r ty x v ** F'.
+Proof.
+  clear. unfold tlocal, tlocal_at.
+  intros.
+  rewrite H.
+  Discharge.discharge fail eauto.
+Qed.
+
+Fixpoint uninitializedN (size : nat) (a : val) : mpred :=
+  match size with
+  | 0 => empSP
+  | S size => (Exists x, ptsto a x) ** uninitializedN size (offset_ptr a 1)
+  end.
+Definition uninitialized (size : N) : val -> mpred :=
+  uninitializedN (BinNatDef.N.to_nat size).
+
+Definition uninitialized_ty (tn : type) (p : val) : mpred :=
+  Exists sz, with_genv (fun g => [| @size_of g tn sz |]) **
+                       uninitialized sz p.
+
+
+(* p is a path
+ * P is a predicate over the resulting value
+ *)
+Definition data (P : val -> mpred) (p : val -> mpred) : mpred.
+refine (Exists v, p v //\\ P v).
+Defined.
+
+Require Import Coq.Lists.List.
+
+Definition tptsto t a v :=
+  _at a (tprim (drop_qualifiers t) v).
+
+Definition tat_field (t : type) (base : val) (f : field) (v : val) : mpred :=
+  _atP base (p_dot f p_done) (tprim t v).
+
+
+
+Lemma tat_uninitialized
+  : forall t b f v F F',
+    F |-- F' ->
+    tat_field t b f v ** F |-- _atP b (p_dot f p_done) (uninit t).
+Proof. Admitted.
